Reduce package count

theories/int_or_ptr/model/int_or_ptr.v
@@ -1,3 +1,0 @@
-From Coq Require Import ZArith.ZArith.
-
-Definition int_or_ptr (X: Type): Type := option (Z + X).
